DynamoDbEncryption/dafny/DynamoDbEncryption/test/Beacon.dfy
@@ -1,13 +1,21 @@
 // Copyright Amazon.com Inc. or its affiliates. All Rights Reserved.
 // SPDX-License-Identifier: Apache-2.0
-include "../../DynamoDbEncryption/src/Beacon.dfy"
-include "../../DynamoDbEncryption/src/CompoundBeacon.dfy"
+include "../src/Beacon.dfy"
+include "../src/CompoundBeacon.dfy"
+include "BeaconTestFixtures.dfy"
+include "../src/ConfigToInfo.dfy"
+include "../src/SearchInfo.dfy"
 
 module TestBaseBeacon {
+  import T = AwsCryptographyDynamoDbEncryptionTypes
   import opened BaseBeacon
   import opened CompoundBeacon
   import opened Wrappers
   import opened TermLoc
+  import opened BeaconTestFixtures
+  import opened DynamoDbEncryptionUtil
+  import C = SearchConfigToInfo
+  import I = SearchableEncryptionInfo
 
   const Timestamp := BeaconPart("timestamp", TermLocMap("timestamp"), "T-", None);
   const Secret := BeaconPart("secret", TermLocMap("secret"), "S-", Some(4));
@@ -45,6 +53,21 @@ module TestBaseBeacon {
     expect str == "80";
     bytes :- expect bb.getHmac(UTF8.EncodeAscii("123"));
     expect bytes[7] == 0x61;
+  }
+
+  method {:test} TestFailures() {
+    var version := T.BeaconVersion (
+      version := 1,
+      key := T.BeaconKey(keyArn := "", tableArn := "", branchKeyID := ""),
+      standardBeacons := None,
+      compoundBeacons := Some([BadPrefix]),
+      virtualFields := None
+    );
+    var beaconVersion :- expect C.ConvertVersionWithKey(FullTableConfig, version, [1,2,3,4,5]);
+
+    var res := beaconVersion.ValidStateResult();
+    expect res.Failure?;
+    expect_equal(res.error, E("Compound beacon BadPrefix defines part Title with prefix T_ which is incompatible with part TooBad which has a prefix of T."));
   }
 
 }
