DynamoDbEncryption/dafny/DynamoDbEncryptionTransforms/src/ExecuteTransactionTransform.dfy
@@ -1,7 +1,7 @@
 // Copyright Amazon.com Inc. or its affiliates. All Rights Reserved.
 // SPDX-License-Identifier: Apache-2.0
 
-include "DdbMiddlewareConfig.dfy"
+include "DynamoDbMiddlewareSupport.dfy"
 include "DdbStatement.dfy"
 
 module ExecuteTransactionTransform {
