DynamoDbEncryption/dafny/DynamoDbEncryptionTransforms/Model/DynamoDbEncryptionTransforms.smithy
@@ -67,6 +67,9 @@ service DynamoDbEncryptionTransforms {
 @aws.polymorph#reference(service: aws.cryptography.dynamoDbEncryption.itemEncryptor#DynamoDbItemEncryptor)
 structure DynamoDbItemEncryptorReference {}
 
+@aws.polymorph#reference(service: aws.cryptography.dynamoDbEncryption#DynamoDbEncryption)
+structure DynamoDbEncryptionReference {}
+
 @error("client")
 structure DynamoDbEncryptionTransformsException {
   @required
